formalize labeled hoare logic with call, some progress in the final theorem

HoareLc_wc.v
@@ -3,16 +3,723 @@ Require Import AST_wc.
 Require Import ASTLc_wc.
 Require Import Hoare_wc.
 
+Require Import Coq.Relations.Relation_Operators.
+Require Import Coq.Relations.Relation_Definitions.
+Arguments clos_refl_trans {A} _ _ _.
+Arguments clos_refl_trans_1n {A} _ _ _.
+Arguments clos_refl_trans_n1 {A} _ _ _.
 
-Definition LContSet := list (label * Assertion).
+Require Import FunctionalExtensionality.
+Require Import ProofIrrelevance.
 
-Definition hoare_triple' (lbc : label_context) (fc' : func_context') (P : LContSet) (c' : com') (Q : LContSet) : Prop :=
-  forall st1 st2 l1 l2 p q,
-    In (l1, p) P ->
-    In (l2, q) Q ->
-    ceval' lbc fc' c' l1 l2 st1 st2 ->
-    p st1 ->
-    q st2.
+Require Import Omega.
 
+Definition top (fc : func_context) (f : func) : lbstk :=
+  (com_to_label_pure (func_bdy f)) :: nil.
+
+Definition bottom (fc : func_context) (f : func) : lbstk :=
+  (com_to_label_pure (func_bdy f)) :: nil.
+
+Inductive matched_label : label -> com -> Prop :=
+  | ML_Skip : matched_label LPure CSkip
+  | ML_Ass : forall X a, matched_label LPure (CAss X a)
+  | ML_Seq : forall l1 l2 c1 c2,
+        matched_label l1 c1 ->
+        matched_label l2 c2 ->
+        matched_label (LSeq l1 l2) (CSeq c1 c2)
+  | ML_If : forall l1 l2 c1 c2 b,
+        matched_label l1 c1 ->
+        matched_label l2 c2 ->
+        matched_label (LIf b l1 l2) (CIf b c1 c2)
+  | ML_While : forall lb c b,
+        matched_label lb c ->
+        matched_label (LWhile b lb) (CWhile b c)
+  | ML_Reentry_here : matched_label LHere CReentry
+  | ML_Reentry_pure : matched_label LPure CReentry.
+
+Definition combine (f1 f2: option func) : option func :=
+  match f1, f2 with
+  | Some f1, None => Some f1
+  | None, Some f2 => Some f2
+  | _, _ => None
+  end.
+
+Fixpoint retrive_func (lb: label) (c: com) : option func :=
+  match lb, c with
+  | LHere, CCall f _ => Some f
+  | LHere, _ => None
+  | LSeq l1 l2, CSeq c1 c2 => combine (retrive_func l1 c1) (retrive_func l2 c2)
+  | LIf _ l1 l2, CIf _ c1 c2 => combine (retrive_func l1 c1) (retrive_func l2 c2)
+  | LWhile _ l1, CWhile _ c1 => retrive_func l1 c1
+  | _, _ => None
+  end.
+
+Fixpoint matched_lbstk (fc: func_context) (bstk: lbstk) (c: com) : Prop :=
+  match bstk with
+  | nil => True
+  | lb :: bstk => single_point lb /\ matched_label lb c /\
+      match bstk, (retrive_func lb c) with
+      | nil, None => True
+      | _, Some f => matched_lbstk fc bstk (func_bdy f)
+      | _, None => False
+      end
+  end.
+
+Definition valid_index_label (fc : func_context) (c : com) (bstk : lbstk) : Prop :=
+  length bstk > 0 /\ matched_lbstk fc bstk c.
+
+Definition Assertion' := state' -> Prop.
+
+Definition A'2A (P: Assertion') : Assertion :=
+  fun (st: state) => match st with
+                     | (loc, glb) => P (loc :: nil, glb)
+                     end.
+
+Definition globalp' (P: Assertion') : Prop :=
+  forall sstk1 sstk2 glb, P (sstk1, glb) -> P (sstk2, glb).
+
+Module COM.
+Definition index_label_set (fc : func_context) (c : com) : Type :=
+  sig (valid_index_label fc c).
+
+Definition rAssertion (fc : func_context) (c : com) : Type :=
+  forall i: index_label_set fc c, Assertion'.
+End COM.
+
+Module FUN.
+Definition index_label_set (fc : func_context) (f : func) : Type :=
+  COM.index_label_set fc (func_bdy f).
+
+Definition rAssertion (fc : func_context) (f : func) : Type :=
+  COM.rAssertion fc (func_bdy f).
+End FUN.
+
+Record index_set (fc : func_context) (lf : list func) : Type := {
+  fname : func;
+  fvalid : In fname lf;
+  index_label : FUN.index_label_set fc fname;
+}.
+
+Definition param_type (fc : func_context) (lf : list func) : Type :=
+  index_set fc lf -> Type.
+
+Definition invariants (fc : func_context) (lf : list func) (pt : param_type fc lf) : Type :=
+  forall i: index_set fc lf, (pt i) -> Assertion'.
+
+Definition index_relation (fc : func_context) (lf : list func) (pt : param_type fc lf) : Type := forall i j : index_set fc lf, (pt i) -> (pt j) -> Prop.
+
+Definition triple_PQ (fc : func_context) (f : func) (P Q : Assertion') (R1 R2 : FUN.rAssertion fc f): Prop :=
+    forall st1 st2,
+      ceval' fc (func_bdy f) (top fc f) (bottom fc f) st1 st2 ->
+      P st1 ->
+      Q st2.
+
+Definition triple_PR (fc : func_context) (f : func) (P Q : Assertion') (R1 R2 : FUN.rAssertion fc f): Prop :=
+    forall st1 st2 (i: FUN.index_label_set fc f),
+      ceval' fc (func_bdy f) (top fc f) (proj1_sig i) st1 st2 ->
+      P st1 ->
+      R2 i st2.
+
+Definition triple_RQ (fc : func_context) (f : func) (P Q : Assertion') (R1 R2 : FUN.rAssertion fc f): Prop :=
+    forall st1 st2 (i: FUN.index_label_set fc f),
+      ceval' fc (func_bdy f) (proj1_sig i) (bottom fc f) st1 st2 ->
+      R1 i st1 ->
+      Q st2.
+
+Definition triple_RR (fc : func_context) (f : func) (P Q : Assertion') (R1 R2 : FUN.rAssertion fc f): Prop :=
+    forall st1 st2 (i1 i2: FUN.index_label_set fc f),
+      ceval' fc (func_bdy f) (proj1_sig i1) (proj1_sig i2) st1 st2 ->
+      R1 i1 st1 ->
+      R2 i2 st2.
+
+Definition func_triple' (fc : func_context) (f : func) (P Q : Assertion') (R1 R2 : FUN.rAssertion fc f): Prop :=
+    triple_PQ fc f P Q R1 R2
+ /\ triple_PR fc f P Q R1 R2
+ /\ triple_RQ fc f P Q R1 R2
+ /\ triple_RR fc f P Q R1 R2.
+
+Inductive reachable_param (fc : func_context) (lf : list func) (f : func) (pt : param_type fc (f :: lf)) (R : index_relation fc (f :: lf) pt) : restk -> forall (i : index_set fc (f :: lf)), (pt i) -> Prop :=
+  | RP_single : forall st i x,
+      fname _ _ i = f ->
+      reachable_param fc lf f pt R ((func_bdy f, Some (proj1_sig (index_label _ _ i)), st) :: nil) i x
+  | RP_multi : forall st1 st2 i j x y stk,
+      In (fname _ _ j) lf ->
+      R i j x y ->
+      reachable_param fc lf f pt R ((func_bdy (fname _ _ i), Some (proj1_sig (index_label _ _ i)), st1) :: stk) i x ->
+      reachable_param fc lf f pt R ((func_bdy (fname _ _ j), Some (proj1_sig (index_label _ _ j)), st2) :: (func_bdy (fname _ _ i), Some (proj1_sig (index_label _ _ i)), st1) :: stk) j y.
+
+Lemma reachable_param_head : 
+  forall fc lf f pt R p stk i x,
+  reachable_param fc lf f pt R (p :: stk) i x ->
+  exists st, p = (func_bdy (fname _ _ i), Some (proj1_sig (index_label _ _ i)), st).
+Proof.
+  intros.
+  inversion H; subst.
+  - exists st.
+    destruct i.
+    simpl in *.
+    subst. auto.
+  - exists st2.
+    auto.
+Qed.
+
+Lemma reachable_param_state :
+  forall fc lf f pt R c l st1 stk i x st2,
+  reachable_param fc lf f pt R ((c, l, st1) :: stk) i x ->
+  reachable_param fc lf f pt R ((c, l, st2) :: stk) i x.
+Proof.
+  intros.
+  remember ((c, l, st1) :: stk) as stk'.
+  induction H; subst.
+  - inversion Heqstk'; subst.
+    apply RP_single.
+    exact H.
+  - inversion Heqstk'; subst.
+    eapply RP_multi.
+    exact H.
+    exact H0.
+    exact H1.
+Qed.
+
+Definition stk_to_pre (fc : func_context) (lf : list func) (f : func) (pt : param_type fc (f :: lf)) (invs : invariants fc (f :: lf) pt) (R : index_relation fc (f :: lf) pt) (stk : restk) (P Q : Assertion') : Prop :=
+  match stk with
+  | nil => False                          (* empty stack *)
+  | (c1, l1, st1) :: stk' =>
+    match stk' with
+    | nil =>                              (* only with bottom level *)
+      match l1 with
+      | Some (l1 :: bstk) =>
+        (is_pure l1 /\ P st1) \/          (* bottom level head *)
+        (single_point l1 /\ exists i x,   (* bottom level reentry *)
+          c1 = func_bdy (fname _ _ i) /\
+          (l1 :: bstk) = proj1_sig (index_label _ _ i) /\
+          reachable_param fc lf f pt R ((c1, Some (l1 :: bstk), st1) :: stk') i x /\
+          invs i x st1)
+      | None => Q st1                     (* bottom level tail *)
+      | _ => False
+      end
+    | _ =>                                (* during reentry *)
+      match l1 with
+      | Some (l1 :: bstk) =>
+        (is_pure l1 /\ exists i x,        (* current level head *)
+          reachable_param fc lf f pt R stk' i x /\ invs i x st1) \/
+        (single_point l1 /\ exists i x,   (* current level reentry *)
+          c1 = func_bdy (fname _ _ i) /\
+          (l1 :: bstk) = proj1_sig (index_label _ _ i) /\
+          reachable_param fc lf f pt R ((c1, Some (l1 :: bstk), st1) :: stk') i x /\
+          invs i x st1)
+      | None => exists i x,               (* current level tail *)
+        reachable_param fc lf f pt R stk' i x /\ invs i x st1
+      | _ => False
+      end
+    end
+  end.
+
+Fixpoint get_bottom_com (stk : restk) : com :=
+  match stk with
+  | nil => CSkip
+  | (c, _, _) :: stk' =>
+    match stk' with
+    | nil => c
+    | _ => get_bottom_com stk'
+    end
+  end.
+
+Lemma ceval'_pure_head :
+  forall fc c l1 l2 st1 st2,
+  is_pure l1 ->
+  ceval' fc c l1 l2 st1 st2 ->
+  l1 = com_to_label_pure c.
+Proof.
+  intros.
+  induction H0; auto;
+  try (inversion H; subst;
+    pose proof IHceval'1 H6;
+    pose proof IHceval'2 H7;
+    subst; auto);
+  try (inversion H; subst;
+    try pose proof IHceval'1 H3;
+    try pose proof IHceval' H4;
+    try pose proof IHceval' H5;
+    try pose proof IHceval' H6;
+    try pose proof IHceval' H7;
+    try pose proof IHceval' H8;
+    subst; auto).
+Qed.
+
+Lemma ceval'_pure_tail :
+  forall fc c l1 l2 st1 st2,
+  is_pure l2 ->
+  ceval' fc c l1 l2 st1 st2 ->
+  l2 = com_to_label_pure c.
+Proof.
+  intros.
+  induction H0; auto;
+  try (inversion H; subst;
+    pose proof IHceval'1 H6;
+    pose proof IHceval'2 H7;
+    subst; auto);
+  try (inversion H; subst;
+    try pose proof IHceval'1 H3;
+    try pose proof IHceval' H4;
+    try pose proof IHceval' H5;
+    try pose proof IHceval' H6;
+    try pose proof IHceval' H7;
+    try pose proof IHceval' H8;
+    subst; auto).
+Qed.
+
+Lemma com_to_label_pure_matched :
+  forall c, matched_label (com_to_label_pure c) c.
+Proof.
+  intros.
+  induction c.
+  - apply ML_Skip.
+  - apply ML_Ass.
+  - apply ML_Seq; assumption.
+  - apply ML_If; assumption.
+  - apply ML_While; assumption.
+  - apply ML_Reentry_pure.
+Qed.
+
+Lemma ceval'_matched_head :
+  forall fc c l1 l2 st1 st2,
+  ceval' fc c l1 l2 st1 st2 ->
+  matched_label l1 c.
+Proof.
+  intros.
+  induction H;
+  try (pose proof (com_to_label_pure_matched c1));
+  try (pose proof (com_to_label_pure_matched c2));
+  try (pose proof (com_to_label_pure_matched c));
+  try (apply ML_Skip);
+  try (apply ML_Ass);
+  try (apply ML_Seq; assumption);
+  try (apply ML_If; assumption);
+  try (apply ML_While; assumption);
+  try constructor.
+  pose proof ceval'_pure_head _ _ _ _ _ _ H H3; subst.
+  exact IHceval'2.
+Qed.
+
+Lemma ceval'_matched_tail :
+  forall fc c l1 l2 st1 st2,
+  ceval' fc c l1 l2 st1 st2 ->
+  matched_label l2 c.
+Proof.
+  intros.
+  induction H;
+  try (pose proof (com_to_label_pure_matched c1));
+  try (pose proof (com_to_label_pure_matched c2));
+  try (pose proof (com_to_label_pure_matched c));
+  try (apply ML_Skip);
+  try (apply ML_Ass);
+  try (apply ML_Seq; assumption);
+  try (apply ML_If; assumption);
+  try (apply ML_While; assumption);
+  try constructor.
+  exact IHceval'2.
+  exact IHceval'2.
+Qed.
+
+
+Lemma multi_ceval'_stack_bottom:
+  forall fc lf stk1 f st,
+    multi_ceval' fc lf stk1 ((func_bdy f, None, st) :: nil) ->
+    get_bottom_com stk1 = func_bdy f.
+Proof.
+  intros.
+  apply Operators_Properties.clos_rt_rt1n in H.
+  remember ((func_bdy f, None, st) :: nil) as stk2.
+  induction H; subst.
+  - auto.
+  - specialize (IHclos_refl_trans_1n (eq_refl _)).
+    inversion H; subst; destruct stk; exact IHclos_refl_trans_1n.
+Qed.
+
+Lemma reentry_bottom_level:
+  forall (fc : func_context) (lf : list func) (f : func) (pt : param_type fc (f :: lf)) (invs : invariants fc (f :: lf) pt) (R : index_relation fc (f :: lf) pt) (P Q : Assertion') (c : com) (l1 : lbstk) (l2 : option lbstk) (st1 st0 : state'),
+
+  (* Rule 2 *)
+  (forall (invs' : FUN.rAssertion fc f),
+    (invs' = fun j st =>
+        exists z, invs {| fname := f; fvalid := in_eq f lf ; index_label := j|} z st) ->
+  func_triple' fc f P Q invs' invs') ->
+
+  get_bottom_com ((c, Some l1, st1) :: nil) = func_bdy f ->
+  stk_to_pre fc lf f pt invs R ((c, Some l1, st1) :: nil) P Q ->
+  middle_ceval' fc lf ((c, Some l1, st1) :: nil) ((c, l2, st0) :: nil) ->
+
+  stk_to_pre fc lf f pt invs R ((c, l2, st0) :: nil) P Q.
+Proof.
+Admitted.
+
+Lemma reentry_higher_level:
+  forall (fc : func_context) (lf : list func) (f : func) (pt : param_type fc (f :: lf)) (invs : invariants fc (f :: lf) pt) (R : index_relation fc (f :: lf) pt) (P Q : Assertion') (c : com) (l1 : lbstk) (l2 : option lbstk) (st1 st0 : state') p stk,
+
+  (* Rule 1 *)
+  (forall f' (Hin: In f' lf) (i: index_set fc (f :: lf)) (x: pt i) invs',
+    (invs' = fun j st =>
+        exists y, R i {| fname := f'; fvalid := in_cons _ _ _ Hin; index_label := j |} x y 
+        /\ invs {| fname := f'; fvalid := in_cons _ _ _ Hin; index_label := j |} y st) ->
+  func_triple' fc f' (invs i x) (invs i x) invs' invs') ->
+
+  (forall (c0 : com) (l : option lbstk) (st : state') (p0 : com * option lbstk * state') (stk' stk'' : restk),
+    (c, Some l1, st1) :: p :: stk = stk' ++ p0 :: stk'' ->
+    In (c0, l, st) stk' -> exists f' : func, In f' lf /\ c0 = func_bdy f') ->
+  stk_to_pre fc lf f pt invs R ((c, Some l1, st1) :: p :: stk) P Q ->
+  middle_ceval' fc lf ((c, Some l1, st1) :: p :: stk) ((c, l2, st0) :: p :: stk) ->
+
+  stk_to_pre fc lf f pt invs R ((c, l2, st0) :: p :: stk) P Q.
+Proof.
+Admitted.
+
+Lemma multi_ceval'_ctop :
+  forall fc lf stk1 c l st p0 p (stk' stk'' : restk),
+    multi_ceval' fc lf (p0 :: nil) stk1 ->
+    stk1 = stk' ++ p :: stk'' ->
+    In (c, l, st) stk' ->
+    exists f', In f' lf /\ c = (func_bdy f').
+Proof.
+Admitted.
+
+Lemma multi_ceval'_left_bottom_single_point :
+  forall fc lf stk c1 c2 l l1 bstk l2 st1 st2,
+  single_point l2 ->
+  multi_ceval' fc lf ((c1, Some (l :: nil), st1) :: nil) (stk ++ (c2, Some (l1 :: bstk ++ l2 :: nil), st2) :: nil) ->
+  single_point l1.
+Proof.
+  intros.
+  remember ((c1, Some (l :: nil), st1) :: nil) as stk1.
+  remember (stk ++ (c2, Some (l1 :: bstk ++ l2 :: nil), st2) :: nil) as stk2.
+  revert H Heqstk2.
+  revert stk c2 l1 bstk l2 st2.
+  apply Operators_Properties.clos_rt_rtn1 in H0.
+  induction H0; intros; subst.
+  - destruct stk; inversion Heqstk2; subst.
+    + app_cons_nil H3.
+    + app_cons_nil H2.
+  - inversion H; subst.
+    + destruct stk; inversion H2; subst.
+      pose proof IHclos_refl_trans_n1 ((c, Some bstk0, st0) :: stk) c2 l1 bstk l2 st2 H1 eq_refl.
+      auto.
+    + destruct stk; inversion H2; subst.
+      * destruct bstk2; inversion H6; subst; [app_cons_nil H8 |].
+        apply app_inj_tail in H8 as [? ?]; subst.
+        eapply ceval'_single_point_stack_right_t2b.
+        exact H3. exact H7.
+      * pose proof IHclos_refl_trans_n1 ((c, Some bstk1, st0) :: stk) c2 l1 bstk l2 st2 H1 eq_refl.
+        auto.
+    + destruct stk; inversion H2; subst.
+      destruct stk; inversion H7; subst.
+      * destruct bstk0; inversion H8; subst; [app_cons_nil H10 |].
+        apply app_inj_tail in H10 as [? ?]; subst.
+        pose proof IHclos_refl_trans_n1 nil c2 l1 bstk l2 (sstk, glb) H1 eq_refl.
+        auto.
+      * pose proof IHclos_refl_trans_n1 ((c0, Some (bstk0 ++ l0 :: nil), (sstk, glb)) :: stk) c2 l1 bstk l2 st2 H1 eq_refl.
+        auto.
+    + destruct stk; inversion H2; subst.
+      * destruct bstk0; inversion H6; subst; [app_cons_nil H8 |].
+        apply app_inj_tail in H8 as [? ?]; subst.
+        pose proof IHclos_refl_trans_n1 ((c0, None, (loc :: nil, glb1)) :: nil) c2 l1 bstk l2 (sstk, glb2) H1 eq_refl.
+        auto.
+      * pose proof IHclos_refl_trans_n1 ((c0, None, (loc :: nil, glb1)) :: (c3, Some (bstk0 ++ l0 :: nil), (sstk, glb2)) :: stk) c2 l1 bstk l2 st2 H1 eq_refl.
+        auto.
+Qed.
+
+Lemma multi_ceval'_left_bottom_bottom_single_point :
+  forall fc lf stk' stk'' c1 c2 l l1 bstk l2 st1 st2,
+  single_point l2 ->
+  multi_ceval' fc lf ((c1, Some (l :: nil), st1) :: nil) (stk' ++ (c2, Some (l1 :: bstk ++ l2 :: nil), st2) :: stk'') ->
+  single_point l1.
+Proof.
+  intros.
+  remember ((c1, Some (l :: nil), st1) :: nil) as stk1.
+  remember (stk' ++ (c2, Some (l1 :: bstk ++ l2 :: nil), st2) :: stk'') as stk2.
+  revert H Heqstk2.
+  revert stk' c2 l1 bstk l2 st2 stk''.
+  apply Operators_Properties.clos_rt_rtn1 in H0.
+  induction H0; intros; subst.
+  - destruct stk'; inversion Heqstk2; subst.
+    + app_cons_nil H3.
+    + pose proof eq_refl (length (stk' ++ (c2, Some (l1 :: bstk ++ l2 :: nil), st2) :: stk'')).
+      rewrite <- H2 in H0 at 1.
+      rewrite app_length in H0.
+      simpl in H0.
+      omega.
+  - inversion H; subst.
+    + destruct stk'; inversion H2; subst.
+      pose proof IHclos_refl_trans_n1 ((c, Some bstk0, st0) :: stk') c2 l1 bstk l2 st2 stk'' H1 eq_refl.
+      auto.
+    + destruct stk'; inversion H2; subst.
+      * destruct bstk2; inversion H6; subst; [app_cons_nil H8 |].
+        apply app_inj_tail in H8 as [? ?]; subst.
+        eapply ceval'_single_point_stack_right_t2b.
+        exact H3. exact H7.
+      * pose proof IHclos_refl_trans_n1 ((c, Some bstk1, st0) :: stk') c2 l1 bstk l2 st2 stk'' H1 eq_refl.
+        auto.
+    + destruct stk'; inversion H2; subst; [app_cons_nil H8 |].
+      destruct stk'; inversion H7; subst.
+      * destruct bstk0; inversion H8; subst; [app_cons_nil H10 |].
+        apply app_inj_tail in H10 as [? ?]; subst.
+        pose proof IHclos_refl_trans_n1 nil c2 l1 bstk l2 (sstk, glb) stk'' H1 eq_refl.
+        auto.
+      * pose proof IHclos_refl_trans_n1 ((c0, Some (bstk0 ++ l0 :: nil), (sstk, glb)) :: stk') c2 l1 bstk l2 st2 stk'' H1 eq_refl.
+        auto.
+    + destruct stk'; inversion H2; subst.
+      * destruct bstk0; inversion H6; subst; [app_cons_nil H8 |].
+        apply app_inj_tail in H8 as [? ?]; subst.
+        pose proof IHclos_refl_trans_n1 ((c0, None, (loc :: nil, glb1)) :: nil) c2 l1 bstk l2 (sstk, glb2) stk'' H1 eq_refl.
+        auto.
+      * pose proof IHclos_refl_trans_n1 ((c0, None, (loc :: nil, glb1)) :: (c3, Some (bstk0 ++ l0 :: nil), (sstk, glb2)) :: stk') c2 l1 bstk l2 st2 stk'' H1 eq_refl.
+        auto.
+Qed.
+
+Theorem reentry_invariant :
+  forall (fc : func_context) (lf : list func) (f : func) (pt : param_type fc (f :: lf)) (invs : invariants fc (f :: lf) pt) (R : index_relation fc (f :: lf) pt) (P Q : Assertion'),
+
+  (forall i x, globalp' (invs i x)) ->
+
+  (* Rule 1 *)
+  (forall f' (Hin: In f' lf) (i: index_set fc (f :: lf)) (x: pt i) invs',
+    (invs' = fun j st =>
+        exists y, R i {| fname := f'; fvalid := in_cons _ _ _ Hin; index_label := j |} x y 
+        /\ invs {| fname := f'; fvalid := in_cons _ _ _ Hin; index_label := j |} y st) ->
+  func_triple' fc f' (invs i x) (invs i x) invs' invs') ->
+
+  (* Rule 2 *)
+  (forall (invs' : FUN.rAssertion fc f),
+    (invs' = fun j st =>
+        exists z, invs {| fname := f; fvalid := in_eq f lf ; index_label := j|} z st) ->
+  func_triple' fc f P Q invs' invs') ->
+
+  func_triple fc lf (A'2A P) f (A'2A Q).
+Proof.
+  unfold A'2A in *.
+  intros.
+  rename H into Ginv.
+  rename H0 into H.
+  rename H1 into H0.
+  unfold func_triple.
+  intros.
+  destruct st1 as [loc1 glb1].
+  destruct st2 as [loc2 glb2].
+  apply ceval_multi_ceval' in H1.
+  remember ((func_bdy f, Some ((com_to_label_pure (func_bdy f)) :: nil), (loc1 :: nil, glb1)) :: nil) as stk1.
+  (* Generalized precondition *)
+  assert (stk_to_pre fc lf f pt invs R stk1 P Q).
+  {
+    subst. simpl.
+    left.
+    split.
+    apply com_to_label_pure_is_pure.
+    exact H2.
+  }
+  remember (func_bdy f, Some (com_to_label_pure (func_bdy f) :: nil), (loc1 :: nil, glb1)) as p'.
+  assert (multi_ceval' fc lf (p' :: nil) stk1) as Hfront.
+  {
+    subst.
+    apply rt_refl.
+  }
+  assert (snd (fst p') = Some (com_to_label_pure (func_bdy f) :: nil)) as Hp'lbstk.
+  {
+    subst.
+    auto.
+  }
+  clear dependent loc1.
+  clear glb1.
+  clear Heqstk1.
+  apply Operators_Properties.clos_rt_rt1n in H1.
+  remember ((func_bdy f, None, (loc2 :: nil, glb2)) :: nil) as stk2.
+  induction H1; intros; subst.
+  - simpl in H3. exact H3.
+  - apply Operators_Properties.clos_rt1n_rt in H2.
+    pose proof multi_ceval'_stack_bottom _ _ _ _ _ H2 as Hbt.
+    specialize (IHclos_refl_trans_1n eq_refl).
+    inversion H1; subst.
+    {
+      apply IHclos_refl_trans_1n; clear IHclos_refl_trans_1n.
+      - destruct stk.
+        (* Transition within the main f, from some point to the end *)
+        * eapply reentry_bottom_level; try assumption.
+          exact H3. assumption.
+        (* Transition in higher level, from some point to the end *)
+        * eapply reentry_higher_level; try assumption.
+          + intros.
+            eapply multi_ceval'_ctop.
+            exact Hfront.
+            exact H5.
+            exact H6.
+          + assumption.
+          + assumption.
+      - apply Operators_Properties.clos_rtn1_rt.
+        eapply rtn1_trans.
+        exact H1.
+        apply Operators_Properties.clos_rt_rtn1.
+        exact Hfront.
+    }
+    {
+      apply IHclos_refl_trans_1n; clear IHclos_refl_trans_1n.
+      - destruct stk.
+        (* Transition with in bottom level, from some point to one reentry point *)
+        * eapply reentry_bottom_level; try assumption.
+          exact H3. assumption.
+        (* Transition within higher level, from some point to one reentry point *)
+        * eapply reentry_higher_level; try assumption.
+          + intros.
+            eapply multi_ceval'_ctop.
+            exact Hfront.
+            exact H6.
+            exact H7.
+          + assumption.
+          + assumption.
+      - apply Operators_Properties.clos_rtn1_rt.
+        eapply rtn1_trans.
+        exact H1.
+        apply Operators_Properties.clos_rt_rtn1.
+        exact Hfront.
+    }
+    {
+      apply IHclos_refl_trans_1n; clear IHclos_refl_trans_1n.
+      (* Transition from lower level to upper level *)
+      - destruct stk.
+          (* (destruct bstk;[
+            simpl in *;
+            destruct H3;[
+              destruct H3;
+              pose proof pure_no_point l1 H3;
+              congruence |
+              left; split;[
+                apply com_to_label_pure_is_pure |
+                destruct H3 as [_ [? [? [? [? [? ?]]]]]];
+                subst; exists x, x0;
+                split; [auto |
+                eapply Ginv;
+                exact H9]]] |
+            assert (single_point l);[
+              destruct p';
+              destruct p;
+              destruct o; inversion Hp'lbstk; subst;
+              eapply multi_ceval'_left_bottom_single_point; [
+              exact H6 |
+              change ((c1, Some ((l :: bstk) ++ l1 :: nil), (sstk, glb)) :: nil) with (nil ++ (c1, Some ((l :: bstk) ++ l1 :: nil), (sstk, glb)) :: nil) in Hfront;
+              exact Hfront]
+            |
+            simpl in *;
+            destruct H3;[
+              destruct H3;
+              pose proof pure_no_point l H3;
+              congruence |
+              left; split;[
+                apply com_to_label_pure_is_pure |
+                destruct H3 as [_ [? [? [? [? [? ?]]]]]];
+                subst; exists x, x0;
+                split; [auto |
+                eapply Ginv;
+                exact H10]]]]]). *)
+        + destruct bstk.
+          {
+            simpl in *.
+            destruct H3.
+            - destruct H3.
+              pose proof pure_no_point l1 H3.
+              congruence.
+            - left; split.
+              * apply com_to_label_pure_is_pure.
+              * destruct H3 as [_ [? [? [? [? [? ?]]]]]].
+                subst; exists x, x0.
+                split; auto.
+                eapply Ginv.
+                exact H9.
+          }
+          {
+            assert (single_point l).
+            {
+              destruct p'.
+              destruct p.
+              destruct o; inversion Hp'lbstk; subst.
+              eapply multi_ceval'_left_bottom_single_point.
+              exact H6.
+              change ((c1, Some ((l :: bstk) ++ l1 :: nil), (sstk, glb)) :: nil) with (nil ++ (c1, Some ((l :: bstk) ++ l1 :: nil), (sstk, glb)) :: nil) in Hfront.
+              exact Hfront.
+            }
+            simpl in *.
+            destruct H3.
+            - destruct H3.
+              pose proof pure_no_point l H3.
+              congruence.
+            - left; split.
+              * apply com_to_label_pure_is_pure.
+              * destruct H3 as [_ [? [? [? [? [? ?]]]]]].
+                subst; exists x, x0.
+                split; auto.
+                eapply Ginv.
+                exact H10.
+          }
+        + destruct bstk.
+          {
+            simpl in *.
+            destruct H3.
+            - destruct H3.
+              pose proof pure_no_point l1 H3.
+              congruence.
+            - left; split.
+              * apply com_to_label_pure_is_pure.
+              * destruct H3 as [_ [? [? [? [? [? ?]]]]]].
+                subst; exists x, x0.
+                split; auto.
+                eapply Ginv.
+                exact H9.
+          }
+          {
+            assert (single_point l).
+            {
+              destruct p'.
+              destruct p0.
+              destruct o; inversion Hp'lbstk; subst.
+              eapply multi_ceval'_left_bottom_bottom_single_point.
+              exact H6.
+              change ((c1, Some ((l :: bstk) ++ l1 :: nil), (sstk, glb)) :: p :: stk) with (nil ++ (c1, Some ((l :: bstk) ++ l1 :: nil), (sstk, glb)) :: p :: stk) in Hfront.
+              exact Hfront.
+            }
+            simpl in *.
+            destruct H3.
+            - destruct H3.
+              pose proof pure_no_point l H3.
+              congruence.
+            - left; split.
+              * apply com_to_label_pure_is_pure.
+              * destruct H3 as [_ [? [? [? [? [? ?]]]]]].
+                subst; exists x, x0.
+                split; auto.
+                eapply Ginv.
+                exact H10.
+          }
+      - apply Operators_Properties.clos_rtn1_rt.
+        eapply rtn1_trans.
+        exact H1.
+        apply Operators_Properties.clos_rt_rtn1.
+        exact Hfront.
+    }
+    {
+      apply IHclos_refl_trans_1n; clear IHclos_refl_trans_1n.
+      (* Transition from upper level to lower level *)
+      - destruct stk; (simpl;
+        destruct H3 as [? [? [? ?]]];
+        right; split; [assumption |
+        exists x, x0;
+        pose proof reachable_param_head _ _ _ _ _ _ _ _ _ H3;
+        destruct H6; inversion H6; subst;
+        repeat split;
+        [eapply reachable_param_state; apply H3|
+         eapply Ginv; exact H5]]).
+      - apply Operators_Properties.clos_rtn1_rt.
+        eapply rtn1_trans.
+        exact H1.
+        apply Operators_Properties.clos_rt_rtn1.
+        exact Hfront.
+    }
+
+Admitted.
 
 
